platform/cito/SetUtil.v
@@ -1,8 +1,0 @@
-Require Import StringSet.
-Import StringSet.
-
-Set Implicit Arguments.
-
-Definition to_set ls := List.fold_left (fun s e => add e s) ls empty.
-
-Definition disjoint a b := forall x, In x a -> In x b -> False.
