platform/cito/SynReqFactsUtil.v
@@ -16,40 +16,24 @@ Qed.
 
 Local Hint Resolve Subset_singleton.
 
-Lemma In_to_set' : forall x ls acc,
-  In x ls \/ StringSet.In x acc
-  -> StringSet.In x (fold_left (fun s e => add e s) ls acc).
-  induction ls; simpl; intuition (subst; eauto).
-  apply IHls.
-  right; apply StringFacts.add_iff; auto.
-  apply IHls.
-  right; apply StringFacts.add_iff; auto.
-Qed.
+Require Import SetoidListFacts.
 
 Lemma In_to_set : forall x ls,
   In x ls
-  -> StringSet.In x (SetUtil.to_set ls).
-  unfold SetUtil.to_set.
-  eauto using In_to_set'.
+  -> StringSet.In x (SSP.of_list ls).
+  intros.
+  eapply SSP.of_list_1.
+  eapply InA_eq_List_In; eauto.
 Qed.
 
 Local Hint Resolve In_to_set.
 
-Lemma to_set_In' : forall x ls acc,
-  StringSet.In x (fold_left (fun s e => add e s) ls acc)
-  -> In x ls \/ StringSet.In x acc.
-  induction ls; simpl; intuition (subst; eauto).
-  apply IHls in H; intuition.
-  apply StringFacts.add_iff in H0; intuition subst.
-Qed.
-
 Lemma to_set_In : forall x ls,
-  StringSet.In x (SetUtil.to_set ls)
+  StringSet.In x (SSP.of_list ls)
   -> In x ls.
-  unfold SetUtil.to_set.
   intros.
-  eapply to_set_In' in H; intuition.
-  apply StringFacts.empty_iff in H0; tauto.
+  eapply SSP.of_list_1 in H.
+  eapply InA_eq_List_In; eauto.
 Qed.
 
 Local Hint Resolve to_set_In.
